\documentclass{physics_notes}

\usepackage{makeidx}
\usepackage{showidx}

\title{Integral Transforms}
%\author{St Aidan's Physics Society}
\date{\today}
\usetikzlibrary{decorations}
\usetikzlibrary{decorations.pathmorphing}
\usetikzlibrary{decorations.markings}
\usetikzlibrary{calc}

\newcommand{\intfty}{\int_{-\infty}^\infty}
\newcommand{\zintfty}{\int_0^\infty}
\newcommand{\F}[2]{\mathcal{F}\left[#1\right](#2)}
\renewcommand{\Finv}[2]{\mathcal{F}^{-1}\left[#1\right](#2)}
\newcommand{\intF}[3]{\frac{1}{\sqrt{2\pi}}\intfty #1 e^{i#3#2}d#2}
\newcommand{\intFinv}[3]{\frac{1}{\sqrt{2\pi}}\intfty #1 e^{-i#3#2}d#3}
\renewcommand{\L}[2]{\mathcal{L}\left[#1\right](#2)}
\newcommand{\Linv}[2]{\mathcal{L}^{-1}\left[#1\right](#2)}
\newcommand{\intL}[3]{\zintfty #1 e^{-#3#2}d#2}

\DeclareMathOperator{\sgn}{sgn}

\makeindex

\begin{document}

\maketitle
\tableofcontents
\newpage

\section*{Introduction}

These notes are based on the Integral Transforms course delivered in Epiphany 2020, by Dr Daniel Cerde√±o. 

There are also frequent references, both explicit and otherwise, made to the book \emph{Mathematical Methods for Physics and Engineering} by K. F. Riley, M. P. Hobson, and S. J. Bence. Relevant chapters of the book are highlighted using coloured square brackets, e.g. \book{24.5}.

Contributors: Ben Amies-King

For a function $f: \mathbb{R} \rightarrow \mathbb{C}$, we define an integral transform:\index{integral transform}

\begin{equation}
g(\omega) = \int_a^b k(\omega, x) f(x) dx
\end{equation}

where the kernel (or propagator) $k(\omega, x)$ is a complex function of two real variables. \index{kernel}

\section{Fourier Transforms}\index{Fourier transform}

We define the Fourier transform, where:

\begin{equation*}
k(\omega, x) = \frac{1}{\sqrt{2\pi}} e^{i\omega x}
\end{equation*}

Hence:

\begin{equation}
\hat{f}(\omega) = \mathcal{F}[f(x)](\omega) = \frac{1}{\sqrt{2\pi}}\int_{-\infty}^\infty f(x) e^{i\omega x} dx
\end{equation}

The condition that $f(x)$ is sufficient to ensure that $\hat{f}(\omega)$ exists. An inverse transform $\mathcal{F}^{-1}: \hat{f} \rightarrow f$ exists if and only if $f$ is continuous. 

Note that the choice of normalisation factor and exponential sign is arbitrary. 

\subsection{Properties of the Fourier transform}

\begin{enumerate}
	\item{
	\begin{align*}
	\mathcal{F}\left[\frac{df}{dx}\right](\omega) &= \frac{1}{\sqrt{2\pi}} \int_{-\infty}^\infty \frac{df}{fx} e^{i\omega x} dx \\
	&= \left.\frac{f e^{i\omega x}}{\sqrt{2\pi}}\right|^{\infty}_{-\infty} - \frac{i\omega}{\sqrt{2\pi}}\int^\infty_{-\infty} f e^{i\omega x} dx \\
	%&= \footnote{0}{As $f$ is square-integrable} - i\omega \mathcal{F}\left[f(x)\right](\omega)
	&= 0 - i\omega \mathcal{F}\left[f(x)\right](\omega)
	\end{align*}
	}
	\item{
	\[\mathcal{F}\left[\frac{d^n f}{dx^n}\right](\omega) = (- i\omega)^n \mathcal{F}\left[f(x)\right](\omega)\]
	}
	\item{
	\begin{align*}
	\mathcal{F}\left[x f(x)\right](\omega) &= \frac{1}{\sqrt{2\pi}} \int_{-\infty}^\infty x f(x) e^{i\omega x} dx \\
	%&\footnote{=}{$\frac{\partial}{\partial\omega}\left(e^{i\omega x}\right) = ixe^{i\omega x}$} \frac{1}{\sqrt{2\pi}} \int_{-\infty}^\infty \frac{f(x)}{i} \frac{\partial}{\partial\omega}\left(e^{i\omega x}\right) dx\\
	&= \frac{1}{\sqrt{2\pi}} \int_{-\infty}^\infty \frac{f(x)}{i} \frac{\partial}{\partial\omega}\left(e^{i\omega x}\right) dx\\
	&= \frac{1}{i}\frac{d}{d\omega} \frac{1}{\sqrt{2\pi}}\int_{-\infty}^{\infty} f(x) e^{i\omega x} dx \\
	&= \frac{1}{i} \frac{d}{d\omega}\mathcal{F}\left[f(x)\right](\omega)
	\end{align*}
	}
	\item{
	\begin{align*}
	\mathcal{F}\left[f(ax)\right](\omega) &= \frac{1}{\sqrt{2\pi}} \int_{-\infty}^\infty f(ax)e^{i\omega x} dx \\
	&= \frac{1}{\sqrt{2\pi}} \int_{-\infty}^\infty f(x') e^{i\frac{\omega}{a}x'} \frac{dx'}{a} \\
	&= \frac{1}{a}\mathcal{F}\left[f(x)\right]\left(\frac{\omega}{a}\right)
	\end{align*}}
	\item{
	\begin{align*}
	\mathcal{F}\left[f(x+a)\right](\omega) &= \frac{1}{\sqrt{2\pi}} \int_{-\infty}^\infty f(x+a)e^{i\omega x} dx \\
	&= e^{-i\omega a}\frac{1}{\sqrt{2\pi}} \int_{-\infty}^\infty f(x') e^{i\omega (x'-a)}dx' \\
	&= e^{-i\omega a}\mathcal{F}\left[f(x)\right]\left(\omega\right)
	\end{align*}}
	\item{
	\begin{align*}
	\mathcal{F}\left[f(x) e^{iax}\right](\omega) &= \frac{1}{\sqrt{2\pi}} \int_{-\infty}^\infty f(x)e^{iax}e^{i\omega x} dx \\
	&= \frac{1}{\sqrt{2\pi}} \int_{-\infty}^\infty f(x) e^{i(a + \omega)x}dx \\
	&=\mathcal{F}\left[f(x)\right]\left(\omega + a\right)
	\end{align*}}
	\item{For $f^\star(x) = f(x)$:
	\begin{align*}
	\left(\mathcal{F}\left[f(x) e^{iax}\right](\omega)\right)^\star &= \left(\frac{1}{\sqrt{2\pi}} \int_{-\infty}^\infty f(x)e^{i\omega x} dx \right)^\star\\
	&= \frac{1}{\sqrt{2\pi}} \int_{-\infty}^\infty f^\star(x)e^{-i\omega x} dx \\
	&= \frac{1}{\sqrt{2\pi}} \int_{-\infty}^\infty f(x)e^{-i\omega x} dx \\
	&=\mathcal{F}\left[f(x)\right](-\omega)
	\end{align*}}
\end{enumerate}

\begin{example}{Wave equation}

\begin{equation*}
\frac{d^2y(x,t)}{dx^2} = \frac{1}{v^2}\frac{d^2y(x,t)}{dt^2}
\end{equation*}

We define \[\mathcal{F}[y(x,t)](k,t) = \hat{y}(k,t)\] so \[\mathcal{F}\left[\frac{d^2y(x,t)}{dx^2}\right](k,t) = (-ik)^2\hat{y}(k,t)\] Hence \[\frac{d^2\hat{y}(k,t)}{dt^2} = -(kv)^2\hat{y}(k,t)\] This yields the solution \[\hat{y}(k,t) = A(k)e^{ikvt} + B(k)e^{-ikvt}\]

We must then transform back into spacial coordinates:

\begin{align*}
y(x,t) &= \mathcal{F}^{-1}\left[A(k)e^{ikvt} + B(k)e^{-ikvt}\right](x,t) \\
&= \frac{1}{\sqrt{2\pi}}\int_{-\infty}^\infty \left(A(k)E^{ikvt} + B(k)e^{-ikvt}\right)e^{-ikx} dk \\
&= \frac{1}{\sqrt{2\pi}}\int_{-\infty}^\infty \left(A(k)E^{-ik(x - vt)} + B(k)e^{-ik(x + vt)}\right)dk \\
\end{align*}
\end{example}


\subsection{$n$-dimensional Fourier transform}

We can generalise this definition to an $n$-dimensional vector space:
\index{n dimensional Fourier transform}
\begin{equation}
\hat{f}(\vec{\omega}) = \frac{1}{(2\pi)^{\frac{n}{2}}} \int_{-\infty}^\infty f(\vec{x}) e^{i\vec{\omega}\cdot\vec{x}} d^n x
\end{equation}


\subsection{Connection to Fourier series}
\index{Fourier series}

Consider a periodic function $f(x)$ over $[-L,L]$. We can write:

\begin{equation}
f(x) = a_0 + \sum_{n=1}^\infty \left(a_n \cos{\frac{n\pi x}{L}} + b_n \sin{\frac{n\pi x}{L}}\right)
\end{equation}

with 

\begin{align*}
a_0 &= \frac{1}{2L}\int_{-L}^{L} f(t) dt \\
a_n &= \frac{1}{L}\int_{-L}^{L} f(t) \cos{\frac{n\pi t}{L}} dt \\
b_n &= \frac{1}{L}\int_{-L}^{L} f(t) \sin{\frac{n\pi t}{L}} dt
\end{align*}

Substituting these expressions into the definiton of the series and applying the identity:

\begin{equation*}
\cos{\frac{n\pi x}{L}}\cos{\frac{n\pi t}{L}} + \sin{\frac{n\pi x}{L}}\sin{\frac{n\pi t}{L}} = \cos{\frac{n\pi}{L}(t-x)}
\end{equation*}

gives

\begin{align*}
f(x) &= \frac{1}{2L}\int_{-L}^{L} f(t)dt + \frac{1}{L}\sum_{n=1}^\infty \int_{-L}^L f(t) \cos{\frac{n\pi}{L}(t-x)} dt \\
&= \frac{1}{2L}\int_{-L}^{L} f(t)dt + \frac{1}{2L}\sum_{n=1}^\infty \int_{-L}^L f(t) \left[ e^{\frac{in\pi}{L}(t-x)} + e^{-\frac{in\pi}{L}(t-x)} \right] dt \\
&= \frac{1}{2L}\int_{-L}^L f(t) e^{\frac{in\pi}{L}(t-x)} \\
\intertext{Defining $\omega_n = \frac{n\pi}{L}$, $\delta\omega = \omega_{n-1} - \omega_n = \frac{\pi}{L}$}
&=\sum_{n=-\infty}^{\infty} \frac{\delta\omega}{2\pi} \int_{-L}^L f(t) e^{i\omega_n t} e^{-i\omega_n x} \\
&\to \frac{1}{\sqrt{2\pi}}\int_{\infty}^\infty \left(\frac{1}{\sqrt{2\pi}} \int_{-\infty}^\infty f(t) e^{i\omega t}dt\right) e^{-i\omega x} d\omega \\
\intertext{as $L\to\infty$}
\end{align*}

\begin{example}{Gaussian function}
Let $f(x) = e^{-\frac{x^2}{2}}$. Then

\begin{align*}
\mathcal{F}\left[f(x)\right](\omega) &= \frac{1}{\sqrt{2\pi}}\int_{-\infty}^\infty e^{-\frac{x^2}{2}} e^{i\omega x} dx \\
&= \frac{1}{\sqrt{2\pi}}\int_{-\infty}^\infty e^{\frac{1}{2}(x - i\omega)^2 - \frac{\omega^2}{2}} dx \\
&= \frac{e^{-\frac{\omega^2}{2}}}{\sqrt{2\pi}}\int_{-\infty}^\infty e^{-\frac{1}{2}(x - i\omega)^2} dx
\end{align*}

For a contour $C_R = C_1 + C_2 + C_3 + C_4$, as $e^{-\frac{z^2}{2}}$ is entire, we have $\oint_{C_R} e^{-\frac{z^2}{2}} = 0$ from Cauchy's theorem.

We need to evaluate 
\[ \lim_{R\to\infty} \left(\int_{C_1} + \int_{C_2} + \int_{C_3} + \int_{C_4}\right)e^{-\frac{z^2}{2}}dz\]

We see 
\begin{align*}
\int_{C_1} e^{-\frac{z^2}{2}} dz &\to \int_{-\infty}^\infty e^{-\frac{x^2}{2}} dx \\
\int_{C_2} e^{-\frac{z^2}{2}} dz &= \int_{C_4} e^{-\frac{z^2}{2}} dz  = 0 \\
\int_{C_3} e^{-\frac{z^2}{2}} dz &\to \int_{-\infty}^\infty e^{-\frac{(x-i\omega)^2}{2}} dx = I
\end{align*}

So $\mathcal{F}\left[e^{-\frac{x^2}{2}}\right] = e^{-\frac{\omega^2}{2}}$, meaning the Fourier transform of a Gaussian is a Gaussian in the transformed variable.
\end{example}

\subsection{Convolutions}

Consider two functions $f(x)$ and $g(x)$ with respective Fourier trasnforms $\hat{f}(\omega)$ and $\hat{g}(\omega)$. We define the convolution of $f$ and $g$ as 

\begin{equation}\label{eq:f_convolution}
f(x) \star g(x) = \frac{1}{\sqrt{2\pi}}\intfty g(y)f(x-y)dy
\end{equation}

We can express $f(x-y$ using the definition of the inverse Fourier transform:

\begin{align*}
f(x) \star g(x) &= \frac{1}{\sqrt{2\pi}} \intfty g(y) \left(\intFinv{\hat{f}{\omega}}{(x-y)}{\omega}\right) \\
&= \intFinv{\hat{f}(\omega) \left(\intF{g(y)}{y}{\omega}\right)}{x}{\omega} \\
&= \intFinv{\hat{f}(\omega)\hat{g}(\omega)}{x}{\omega} \\
&= \Finv{\hat{f}(\omega)\hat{g}(\omega)}{x} \\
\intertext{Applying the Fourier transform to both sides:} \\
\F{f(x) \star g(x)}{\omega} &= \hat{f}(\omega)\hat{g}(\omega)
\end{align*}

\begin{example}{}
Consider the differential equation \[f''(x) - f(x) = e^{-x^2}\] The homogeneous solution is \[f_0(x) = Ae^x + Be^{-x}\]

The third particular solution can be found by applying the Fourier transform to each side:
\begin{align*}
\F{f''(x) - f(x)}{\omega} &= \F{e^{-x^2}}{\omega} \\
(-i\omega)^2\hat{f}(\omega) - \hat{f}(\omega) &= \F{e^{-x^2}}{\omega} \\
\hat{f}(\omega) &= -\frac{1}{1+\omega^2}\cdot\F{e^{-x^2}}{\omega} \\
\intertext{So by application of the convolution theorem:} \\
f(x) &= -e^{-x^2} \star \Finv{\frac{1}{1+\omega^2}}{x}
\end{align*}

We can evaluate the inverse Fourier transform using complex analysis, by considering a contour:

\begin{equation*}
C_R = \begin{cases}[0,R]\cup\left\{\frac{R}{2}\left(1 + e^{i\theta}\right)\right\},\theta\in\left[0,-\pi\right) & \text{ for } x \geq 0 \\ [-R,0]\cup\left\{\frac{R}{2}\left(-1 + e^{i\theta}\right)\right\},\theta\in\left[0,\pi\right) & \text{ for } x <\geq> 0 \end{cases}
\end{equation*}

This leads to

\begin{align*}
\Finv{\frac{1}{1+\omega^2}}{x} &= \intFinv{\frac{1}{1+\omega^2}}{x}{\omega} \\
&= \frac{1}{\sqrt{2\pi}} 2\pi i\left(\left.-Res\left[\frac{e^{-i\omega x}}{1+\omega^2}\right]_{x=-i}\right|_{x\geq 0} + \left.Res\left[\frac{e^{-i\omega x}}{1+\omega^2}\right]_{x=i}\right|_{x < 0} \right) \\
&= \sqrt{\frac{\pi}{2}}\left(\left.e^{-x}\right|_{x\geq 0} + \left. e^x\right|_{x<0}\right) \\
&= \sqrt{\frac{\pi}{2}}e^{|x|}
\end{align*}

So 
\begin{align*}
f(x) &= -e^{-x^2} \star \sqrt{\frac{\pi}{2}}e^{-|x|} \\
&= -\frac{1}{2}\intfty e^{-(x-y)^2}e^{-|y|} dy
\end{align*}
\end{example}

\subsection{Parseval's Theorem}

\begin{theorem}{Parseval's Theorem}
$\intfty f^\star(x)g(x)dx = \intfty \hat{f}(\omega)\hat{g}(\omega)d\omega$
\end{theorem}

We see, using a property of the Dirac $\delta$-function \ref{sec:dirac_delta}:

\begin{align*}
\intfty f^\star(x)g(x)dx &= \intfty \left(\Finv{\hat{f}(\omega)}{x}\right)^\star \Finv{\hat{g}(\omega)}{x} dx \\
&= \frac{1}{2\pi}\intfty dx \intfty \hat{f}^\star(\omega)e^{i\omega x} d\omega \intfty \hat{g}(\omega') e^{-i\omega' x} d\omega' \\
&= \intfty \intfty \intfty dx d\omega d\omega' \hat{f}^\star (\omega) \hat{g}(\omega') e^{-ix(\omega' - \omega)}
&= \intfty \intfty d\omega d\omega' \hat{f}^\star(\omega) \hat{g}(\omega') \delta(\omega' - \omega) \\
&= \intfty \hat{f}^\star(\omega)g(\omega) d\omega
\end{align*}

Note that if we take $g(x) = f(x)$, the Parseval theorem shows that normalisation is consered by the Fourier transform.

The Fourier transform is thus a unitary operation in the Hilbert space $\mathbb{L}^2$ of square-integrable functions, and the PArseval theorem is a manifestation of this property.

\begin{example}{$I = \int_{0}^\infty \frac{d\omega}{(a^2 + \omega^2)^2}$}

Define $k = \frac{\omega}{a}$. Thus:

\[ I \to \frac{1}{2a^3}\intfty \frac{dk}{(1 + k^2)^2} \]

We know $\Finv{\frac{1}{1+k^2}}{x} = \sqrt{\frac{\pi}{2}} e^{|x|}$, hence by Parseval's theorem:

\begin{align*}
\intfty \frac{dk}{(1+k^2)^2} &= \intfty \left(\sqrt{\frac{\pi}{2}}e^{-|x|}\right)^2 dx \\
&= \pi\int_{0}^\infty e^{-2x} dx \\
&= \frac{\pi}{2}
\end{align*}

So $I = \frac{\pi}{4a^3}$
\end{example}



\subsection{Solving Integral Equations}

The Fourier transform can also be used to solve integral equations that involve convolution of functions. Consider

\[ h(x) = e^{i3x} + \intfty e^{-|y|}h(x-y)dy \]

Noticing that the integral on the right-hand side is a convolution, we can apply the Fourier transform to obtain

\begin{align*}
\hat{h}(\omega) &= \sqrt{2\pi} \delta(\omega + 3) + \frac{2}{1+w^2} \hat{h}(\omega) \\
\intertext{ which can be written }
&= \sqrt{2\pi} \delta(\omega + 3)\left(1 + \frac{2}{1+w^2} \hat{h}(\omega)\right)^{-1}
\end{align*}

Inverting this relation gives
\begin{align*}
h(x) &= \intF{\sqrt{2\pi} \delta(\omega + 3)\left(1 + \frac{2}{1+w^2} \hat{h}(\omega)\right)^{-1}}{x}{\omega} \\
&= \frac{5}{4}e^{i3x}
\end{align*}

\subsection{Discrete Fourier Transforms} \index{discrete Fourier transform}

For a function $h(t)$ with period $T$, we can perform a set of measurements $h_j$ within a period. We will consider $h_j$ to be an even number of points $2N$ sampled at times $t_j = j\frac{T}{2N}$.

The discrete Fourier transform (DFT) for this set of data is

\begin{equation}\label{eq:dft}
\hat{h}(\omega_p) = \frac{1}{\sqrt{2N}}\sum_{j=0}^{2N-1} h_j e^{i\omega_p t_j}
\end{equation}

where $\omega_p = \frac{2\pi p}{T}$ with $0 \leq p \leq 2N-1$.

Notice that this decomposition includes as many frequencies as time measurements were performed. We can invert this relation:

\begin{equation*}\label{eq:inv_dft}
h^{DFT}(t) = \frac{1}{\sqrt{2N}}\sum_{p=0}^{2N-1} \hat{h}_p e^{-i\omega_p t}
\end{equation*}

Note that $h^{DFT}$ is defined for all $t$, with $h^{DFT} \to h$ as $N\to\infty$.

\subsection{The Fourier Matrix}\index{Fourier matrix}

We can express the above procedure in terms of the Fourier matrix:

\begin{equation*}
\begin{pmatrix} \hat{h}_1 \\ \vdots \\ \hat{h}_{2N-1} \end{pmatrix} = F(2N)_{p_j} \begin{pmatrix} h_1 \\ \vdots \\ h_{2N-1} \end{pmatrix}
\end{equation*}

where
\begin{equation}
F(2N)_{p_j} = \left(\frac{e^{i\omega_p t_j}}{\sqrt{2N}}\right) = \left(\frac{e^{i\pi p j/N}}{\sqrt{2N}}\right)
\end{equation}
is the Fourier matrix which provides the basis of plane waves in which the signal is expanded.

\begin{example}{}
Consider the periodic signal $h(t) = \cos{t}$, with period $T = 2\pi$. Using the following measurements, N = 2:


\begin{tabular}{c || c | c | c}
$t$ & $h(t)$ & $p$ & $\omega_p$ \\
\hline
$0$ & $1$ & $0$ & $\frac{0}{T} = 0$ \\
$\frac{\pi}{2}$ & $0$ & $1$ & $\frac{2\pi}{T} = 1$ \\
$\pi$ & $-1$ & $2$ & $\frac{4\pi}{T} = 2$ \\
$\frac{3\pi}{2}$ & $0$ & $3$ & $\frac{6\pi}{T} = 3$
\end{tabular}

So

\begin{equation*}
\begin{pmatrix} \hat{h}_0 \\ \hat{h}_1 \\ \hat{h}_2 \\ \hat{h}_3 \end{pmatrix} = \frac{1}{2}\begin{pmatrix} 1 & 1 & 1 & 1 \\ 1 & i & -1 & -i \\ 1 & -1 & 1 & -1 \\ 1 & -i & -1 & i\end{pmatrix}\begin{pmatrix} 1 \\ 0 \\ -1 \\ 0\end{pmatrix}
\end{equation*}

We can now apply the inverse DFT to obtain

\begin{align*}
\hat{h}(t) &= \frac{1}{2}\sum_{p=0}^{2N-1} \hat{h}_p e^{-i\omega_p t} \\
&= \frac{1}{2}\left( 0\cdot e^{-0\cdot it} + 1\cdot e^{-1\cdot it} + 0\cdot e^{-2\cdot it} + 1\cdot e^{-3\cdot it}\right) \\
\intertext{Given that the function is real:} \\
h(t) &= \frac{1}{2}\left(\cos{t} + \cos{3t}\right)
\end{align*}
\end{example}

\section{Laplace Transforms} \index{Laplace transform}

The Laplace transform is an integral transform with kernel $k(t,s) = e^{-ts}$, defined:

\begin{equation}
\L{f(t)}{s} \equiv \bar{f}(s) = \intL{f(t)}{t}{s}
\end{equation}

which is typically defined for $s>0$.

We have the following standard results:

\begin{enumerate}
	\item{}
\end{enumerate}

\begin{example}{}
\begin{align*}
\L{1}{s} &= \intL{1}{t}{s} \\
&= \frac{1}{s} \, s>0
\end{align*}
\end{example}

\begin{example}{}
\begin{align*}
\L{e^{at}}{s} &= \intL{e^{at}}{t}{s} \\
&= \zintfty e^{-(s-a)t} dt \\
&= \frac{1}{s-a} \, s>a
\end{align*}
\end{example}

\subsection{Link to Fourier Transform}

We can relate the Laplace transform to the Fourier transform by assuming $s=x+iy$:

\begin{align}
\L{f(t)}{s} &= \intL{f(t)}{t}{s} \nonumber \\
&= \zintfty f(t) e^{-(x+iy)t} dt \nonumber \\
&= \zintfty f(t) e^{-xt} e^{-iyt} dt \nonumber \\
&= \intfty f(t) e^{-xt} H(t)e^{iyt} dt \nonumber \\
&= \Finv{f(t)H(t)e^{-xt}}{y}
\end{align}

\begin{example}{}
\begin{align*}
\L{\frac{df}{dt}}{s} &= \intL{\frac{df}{dt}}{t}{s} \\
&= \underbrace{\left. f(t)e^{-st}\right|^\infty_0}{-f(0) \text{ by convergence.}} - \zintfty f(t)\frac{\partial e^{-st}}{\partial t} dt \\
&= -f(0) + s\zintfty f(t) e^{-st} dt \\
&= s\L{f(t)}{s} - f(0)
\end{align*}
\end{example}

In general:
\begin{equation*}
\L{\frac{d^n f}{dt^n}}{s} = s^n\L{f(t)}{s} - \sum_{k=0}^{n-1} s^{n-1-k}f^{(k)}(0)
\end{equation*}

\begin{example}{$f(t) = \sinh{kt} = \frac{1}{k}\frac{\partial \cosh{kt}}{\partial t}$}
\begin{align*}
\L{\sinh{kt}}{s} &= \frac{1}{k}\L{\frac{\partial}{\partial t}\cosh{kt}}{s} \\
&= \frac{s}{k}\L{\cosh{kt}}{s} - \frac{1}{k}\cosh{0} \\
&= \frac{1}{k}\left(\frac{s^2}{s^2 - k^2} - 1\right) \\
&= \frac{k}{s^2 - k^2} \, s>|k|
\end{align*}
\end{example}

The Laplace transform can also be a useful tool in solving integrals.

\begin{example}{$f(t) = \zintfty \frac{\sin{tx}}{x}dx$}
\begin{align*}
\bar{f}(s) &= \L{\zintfty \frac{\sin{tx}}{x}}{s} \\
&= \zintfty dt \zintfty\frac{\sin{tx}}{x}e^{-st} dx \\
&= \zintfty \L{\sin{tx}}{s}\frac{dx}{x} \\
&= \zintfty \frac{1}{s^2 + x^2} dx \\
&= \frac{\pi}{2s}
\end{align*}

So for $t>0$ we have $f(t) = \frac{\pi}{2}$. For $t<0$ we use $\sin{-t} = -\sin{t}$ to obtain $f(t) = -\frac{\pi}{2}$. Hence $f(t) = \frac{\pi}{2}\sgn{t}$
\end{example}


\subsection{Laplace Transforms of Periodic Functions}


\section{The Dirac $\delta$-function}\label{sec:dirac_delta}

The Dirac $\delta$-function is commonly defined as follows:

\begin{enumerate}
	\item $\delta(x) = 0$ if $x\neq 0$
	\item $\int_{-\infty}^\infty \delta(x) dx = 1$
	\item $\int_{-\infty}^\infty \delta(x) f(x) dx = f(0)$
\end{enumerate}

In order to obtain a more rigorous definition, we consider a sequence of functions:

\begin{equation*}
f_n = \frac{n}{\sqrt{\pi}}e^{-n^2x^2}
\end{equation*}

As $n\to\infty$, $f_n$ replicates the behaviour of the $\delta$-function.

Similarly, we can define it as the limit as $n\to\infty$ of

\begin{equation*}
g_n(x) = \frac{n}{\pi}\frac{1}{1+n^2x^2}
\end{equation*}

We see:

\begin{enumerate}
	\item{\[\lim_{n\to\infty}g_n(x) = \begin{cases} 0 & \text{ if } x\neq0 \\ \infty & \text{ if } x=0\end{cases}\]}
	\item{
	\begin{align*} \lim_{n\to\infty}\int_{-\infty}^\infty g_n(x)dx &= \lim_{n\to\infty}\int_{-\infty}^\infty \frac{n}{\pi}\frac{1}{1+n^2x^2}dx \\
	&= \frac{2\cancel{\pi} i}{\cancel{\pi}}Res\left(\frac{1}{n^2(z+\frac{i}{n})(z-\frac{i}{n})}\right)_{z=\frac{i}{n}} \\
	&= 1
	\end{align*}}
	\item{
	\begin{align*} \lim_{n\to\infty}\int_{-\infty}^\infty g_n(x)f(x)dx &= \lim_{n\to\infty}\int_{-\infty}^\infty \frac{n}{\pi}\frac{f(x)}{1+n^2x^2}dx \\
	&= \frac{2\cancel{\pi} i}{\cancel{\pi}}Res\left(\frac{f(x)}{n^2(z+\frac{i}{n})(z-\frac{i}{n})}\right)_{z=\frac{i}{n}} \\
	&= f\left(\frac{i}{n}\right) \stackrel{n\to\infty}{\longrightarrow} f(0)
	\end{align*}}
\end{enumerate}

There are many other similar sequences of functions which we could use. The fact that we must define the Dirac $\delta$-function in this way means that it is a distribution.

\subsection{Properties of the Dirac $\delta$-function}
\begin{enumerate}
	\item{$\delta(-x) = \delta(x)$}
	\item{$\delta(x-a)f(x) = \delta(x-a)f(a)$ if $f$ is continuous at $x=a$}
	\item{If a function $g(x)$ has at most simple zeros $x_i$ then \begin{equation*}\delta(g(x)) = \sum_{x_i} \frac{\delta(x-x_i)}{\left|g'(x_i)\right|}\end{equation*}}
	\item{$\delta(ax) = \frac{\delta(x)}{\|a\|}$}
	\item{The Dirac $\delta$-function is differentiable, with: \begin{align*}\int_{-\infty}^\infty \delta '(x)f(x)dx &= \left. f(x)\delta(x)\right|_{-\infty}^\infty - \int_{-\infty}^\infty \delta(x) f'(x) dx \\ &= -f'(0) \\ \intertext{where $f(x)$ vanishes at $\pm\infty$. Similarly, for higher orders:} \intfty \delta^n (x)f(x)dx = (-1)^n f^{(n)}(0) \end{align*}}
	\item{$H'(x) = \delta(x)$, where $H(x)$ is the Heaviside step function, defined: \begin{equation} H(x) = \begin{cases} 1 & x\geq 0 \\ 0 & x < 0 \end{cases}\end{equation}}
\end{enumerate}
\subsection{Fourier Representation of the Dirac $\delta$-function}

We see:

\begin{align*}
\F{\delta(x)}{\omega} &= \intF{x}{\omega}{\delta(x)} \\
&= \frac{1}{\sqrt{2\pi}}
\end{align*}

Applying the inverse transform, we obtain:
\begin{align*}
\Finv{\hat{\delta}(\omega)}{x} &= \intFinv{x}{\omega}{\frac{1}{\sqrt{2\pi}}} \\
&= \frac{1}{2\pi}\intfty{e^{-i\omega x} d\omega}
\end{align*}

So we can show:
\begin{enumerate}
	\item{$\F{1}{\omega} = \sqrt{2\pi}\delta(\omega)$}
	\item{$\F{e^{i\alpha x}}{\omega} = \intF{e^{i\alpha x}}{x}{\omega} = \sqrt{2\pi}\delta(\omega + \alpha)$}
\end{enumerate}


\newpage
\printindex
\end{document}